feat: fix/weakening

CollapsingTowers/TwoLevelRec/Syntax/SyntacticTrans.lean
@@ -68,3 +68,35 @@ def maping𝕔 (i : ℕ) (e : Expr) : Expr :=
   | .fix𝕔 e => .fix𝕔 (maping𝕔 (i + 2) e)
   | .lets b e => .lets (maping𝕔 i b) (maping𝕔 (i + 1) e)
   | .lets𝕔 b e => .lets𝕔 (maping𝕔 i b) (maping𝕔 (i + 1) e)
+
+@[simp]
+def shiftl_at (x : ℕ) (n : ℕ) : Expr → Expr
+  | .bvar i => .bvar i
+  | .fvar y => if x ≤ y then .fvar (y + n) else .fvar y
+  | .fix e => .fix (shiftl_at x n e)
+  | .lift e => .lift (shiftl_at x n e)
+  | .app₁ f arg => .app₁ (shiftl_at x n f) (shiftl_at x n arg)
+  | .app₂ f arg => .app₂ (shiftl_at x n f) (shiftl_at x n arg)
+  | .lit n => .lit n
+  | .run e => .run (shiftl_at x n e)
+  | .code e => .code (shiftl_at x n e)
+  | .reflect e => .reflect (shiftl_at x n e)
+  | .fix𝕔 e => .fix𝕔 (shiftl_at x n e)
+  | .lets b e => .lets (shiftl_at x n b) (shiftl_at x n e)
+  | .lets𝕔 b e => .lets𝕔 (shiftl_at x n b) (shiftl_at x n e)
+
+@[simp]
+def shiftr_at (x : ℕ) : Expr → Expr
+  | .bvar i => .bvar i
+  | .fvar y => if x < y then .fvar (y - 1) else .fvar y
+  | .fix e => .fix (shiftr_at x e)
+  | .lift e => .lift (shiftr_at x e)
+  | .app₁ f arg => .app₁ (shiftr_at x f) (shiftr_at x arg)
+  | .app₂ f arg => .app₂ (shiftr_at x f) (shiftr_at x arg)
+  | .lit n => .lit n
+  | .run e => .run (shiftr_at x e)
+  | .code e => .code (shiftr_at x e)
+  | .reflect e => .reflect (shiftr_at x e)
+  | .fix𝕔 e => .fix𝕔 (shiftr_at x e)
+  | .lets b e => .lets (shiftr_at x b) (shiftr_at x e)
+  | .lets𝕔 b e => .lets𝕔 (shiftr_at x b) (shiftr_at x e)
