CollapsingTowers/TwoLevelRec/SyntacticTyping/Weakening.lean
@@ -1,0 +1,120 @@
+import CollapsingTowers.TwoLevelRec.SyntacticTyping.Typing
+
+theorem typing.weakening.strengthened :
+    ∀ Γ Ψ Δ Φ 𝕊 e τ φ,
+      typing Γ 𝕊 e τ φ →
+      Γ = Ψ ++ Φ →
+      typing (Ψ ++ Δ ++ Φ) 𝕊 (shiftl_at Φ.length Δ.length e) τ φ :=
+  by
+  intros Γ Ψ Δ Φ 𝕊 e τ φ Hτ HEqΓ
+  revert Ψ
+  apply
+    @typing.rec
+      (fun Γ 𝕊 e τ φ (H : typing Γ 𝕊 e τ φ) =>
+        ∀ Ψ,
+          Γ = Ψ ++ Φ →
+          typing (Ψ ++ Δ ++ Φ) 𝕊 (shiftl_at Φ.length Δ.length e) τ φ)
+      (fun Γ e τ φ (H : typing_reification Γ e τ φ) =>
+        ∀ Ψ,
+          Γ = Ψ ++ Φ →
+          typing_reification (Ψ ++ Δ ++ Φ) (shiftl_at Φ.length Δ.length e) τ φ)
+  <;> intros
+  case fvar x _ Hbinds Hwbt Ψ HEqΓ =>
+    rw [HEqΓ] at Hbinds
+    by_cases HLe : Φ.length <= x
+    . simp only [shiftl_at]; rw [if_pos HLe]; apply typing.fvar
+      rw [← Nat.add_sub_of_le HLe]
+      rw [← Nat.add_sub_of_le HLe] at Hbinds
+      rw [Nat.add_assoc, Nat.add_left_comm, ← Nat.add_assoc, Nat.add_right_comm]
+      rw [Nat.add_comm] at Hbinds
+      repeat apply binds.extendr
+      apply binds.shrinkr; apply Hbinds; apply Hwbt
+    . simp only [shiftl_at]; rw [if_neg HLe]; apply typing.fvar
+      apply binds.extend; apply binds.shrink
+      omega; apply Hbinds; apply Hwbt
+  case fix Hwbt Hclose IH Ψ HEqΓ =>
+    rw [HEqΓ] at IH Hclose
+    have HEq₀ : (Ψ ++ Δ ++ Φ).length = (Ψ ++ Φ).length + Δ.length := by simp; omega
+    have HEq₁ : (Ψ ++ Δ ++ Φ).length + 1 = (Ψ ++ Φ).length + 1 + Δ.length := by simp; omega
+    rw [comm.shiftl_opening, comm.shiftl_opening] at IH
+    apply typing.fix
+    rw [← List.cons_append, ← List.cons_append, ← List.cons_append, ← List.cons_append]
+    rw [HEq₁, HEq₀]; apply IH; rfl; apply Hwbt
+    rw [HEq₀]; apply closed.under_shiftl; apply Hclose
+    simp; simp; omega
+  case lift_lam IH Ψ HEqΓ =>
+    apply typing.lift_lam
+    apply IH; apply HEqΓ
+  case fix𝕔 Hwbt Hclose IH Ψ HEqΓ =>
+    rw [HEqΓ] at IH Hclose
+    have HEq₀ : (Ψ ++ Δ ++ Φ).length = (Ψ ++ Φ).length + Δ.length := by simp; omega
+    have HEq₁ : (Ψ ++ Δ ++ Φ).length + 1 = (Ψ ++ Φ).length + 1 + Δ.length := by simp; omega
+    rw [comm.shiftl_opening, comm.shiftl_opening] at IH
+    apply typing.fix𝕔
+    rw [← List.cons_append, ← List.cons_append, ← List.cons_append, ← List.cons_append]
+    rw [HEq₁, HEq₀]; apply IH; rfl; apply Hwbt
+    rw [HEq₀]; apply closed.under_shiftl; apply Hclose
+    simp; simp; omega
+  case app₁ IHf IHarg Ψ HEqΓ =>
+    apply typing.app₁
+    apply IHf; apply HEqΓ
+    apply IHarg; apply HEqΓ
+  case app₂ IHf IHarg Ψ HEqΓ =>
+    apply typing.app₂
+    apply IHf; apply HEqΓ
+    apply IHarg; apply HEqΓ
+  case lit => apply typing.lit
+  case lift_lit IH Ψ HEqΓ =>
+    apply typing.lift_lit
+    apply IH; apply HEqΓ
+  case code_fragment x _ Hbinds Hwbt Ψ HEqΓ =>
+    rw [HEqΓ] at Hbinds
+    by_cases HLe : Φ.length <= x
+    . simp only [shiftl_at]; rw [if_pos HLe]; apply typing.code_fragment
+      rw [← Nat.add_sub_of_le HLe]
+      rw [← Nat.add_sub_of_le HLe] at Hbinds
+      rw [Nat.add_assoc, Nat.add_left_comm, ← Nat.add_assoc, Nat.add_right_comm]
+      rw [Nat.add_comm] at Hbinds
+      repeat apply binds.extendr
+      apply binds.shrinkr; apply Hbinds; apply Hwbt
+    . simp only [shiftl_at]; rw [if_neg HLe]; apply typing.code_fragment
+      apply binds.extend; apply binds.shrink
+      omega; apply Hbinds; apply Hwbt
+  case code_rep IH Ψ HEqΓ =>
+    apply typing.code_rep
+    apply IH; apply HEqΓ
+  case reflect IH Ψ HEqΓ =>
+    apply typing.reflect
+    apply IH; apply HEqΓ
+  case lets Hwbt Hclose IHb IHe Ψ HEqΓ =>
+    rw [HEqΓ] at IHe Hclose
+    have HEq : (Ψ ++ Δ ++ Φ).length = (Ψ ++ Φ).length + Δ.length := by simp; omega
+    rw [comm.shiftl_opening] at IHe
+    apply typing.lets
+    apply IHb; apply HEqΓ
+    rw [← List.cons_append, ← List.cons_append]
+    rw [HEq]; apply IHe; rfl; apply Hwbt
+    rw [HEq]; apply closed.under_shiftl; apply Hclose
+    simp
+  case lets𝕔 Hwbt Hclose IHb IHe Ψ HEqΓ =>
+    rw [HEqΓ] at IHe Hclose
+    have HEq : (Ψ ++ Δ ++ Φ).length = (Ψ ++ Φ).length + Δ.length := by simp; omega
+    rw [comm.shiftl_opening] at IHe
+    apply typing.lets𝕔
+    apply IHb; apply HEqΓ
+    rw [← List.cons_append, ← List.cons_append]
+    rw [HEq]; apply IHe; rfl; apply Hwbt
+    rw [HEq]; apply closed.under_shiftl; apply Hclose
+    simp
+  case run Hclose IH Ψ HEqΓ =>
+    apply typing.run
+    apply IH; apply HEqΓ
+    rw [identity.shiftl]; apply Hclose
+    apply closed.inc; apply Hclose; omega
+  case pure IH Ψ HEqΓ =>
+    apply typing_reification.pure
+    apply IH; apply HEqΓ
+  case reify IH Ψ HEqΓ =>
+    apply typing_reification.reify
+    apply IH; apply HEqΓ
+  apply Hτ
