CollapsingTowers/TwoLevelRec/Syntax/Commutative.lean
@@ -1,0 +1,27 @@
+import CollapsingTowers.TwoLevelRec.Syntax.Identity
+
+lemma comm.shiftl_opening : ∀ x y e n i, x ≤ y → (shiftl_at x n {i ↦ y} e) = ({i ↦ y + n} shiftl_at x n e) :=
+  by
+  intros x y e n i HLe
+  induction e generalizing i with
+  | bvar j =>
+    by_cases HEq : j = i
+    . rw [HEq]; simp; omega
+    . simp; rw [if_neg HEq]; rw [if_neg HEq]; rfl
+  | fvar z =>
+    by_cases HLe : x ≤ z
+    . simp; rw [if_pos HLe]; rfl
+    . simp; rw [if_neg HLe]; rfl
+  | app₁ _ _ IH₀ IH₁
+  | app₂ _ _ IH₀ IH₁
+  | lets _ _ IH₀ IH₁
+  | lets𝕔 _ _ IH₀ IH₁ =>
+    simp; constructor; apply IH₀; apply IH₁
+  | lit => simp
+  | fix _ IH
+  | lift _ IH
+  | fix𝕔 _ IH
+  | code _ IH
+  | reflect _ IH
+  | run _ IH =>
+    simp; apply IH
