CollapsingTowers/TwoLevelRec/Syntax/Defs.lean
@@ -2,3 +2,5 @@ import CollapsingTowers.TwoLevelRec.Syntax.Effect
 import CollapsingTowers.TwoLevelRec.Syntax.Basic
 import CollapsingTowers.TwoLevelRec.Syntax.SyntacticTrans
 import CollapsingTowers.TwoLevelRec.Syntax.Closedness
+import CollapsingTowers.TwoLevelRec.Syntax.Identity
+import CollapsingTowers.TwoLevelRec.Syntax.Commutative
