CollapsingTowers/TwoLevelRec/Syntax/Identity.lean
@@ -1,0 +1,24 @@
+import CollapsingTowers.TwoLevelRec.Syntax.Closedness
+
+lemma identity.shiftl :
+    ∀ x e n, closed_at e x → shiftl_at x n e = e :=
+  by
+  intros x e n
+  induction e with
+  | bvar j => simp
+  | fvar y => simp; omega
+  | app₁ _ _ IH₀ IH₁
+  | app₂ _ _ IH₀ IH₁
+  | lets _ _ IH₀ IH₁
+  | lets𝕔 _ _ IH₀ IH₁ =>
+    intro Hclosed; simp; constructor
+    apply IH₀; apply Hclosed.left
+    apply IH₁; apply Hclosed.right
+  | lit => simp
+  | fix _ IH
+  | lift _ IH
+  | fix𝕔 _ IH
+  | code _ IH
+  | reflect _ IH
+  | run _ IH =>
+    simp; apply IH
